src/PlutusIR/Semantics/Static/NormalisationSS.v
@@ -1,0 +1,1083 @@
+From Equations Require Import Equations.
+Require Import PlutusCert.PlutusIR.
+Require Import Strings.String.
+Require Export PlutusCert.PlutusIR.Semantics.Static.Kinding.
+Require Export PlutusCert.PlutusIR.Semantics.Static.TypeSubstitution.
+Require Import List.
+Import ListNotations.
+From PlutusCert Require Import Analysis.FreeVars.
+Import Ty.
+Require Import Bool.
+Require Import PlutusCert.Util.Map.
+Require Import PlutusCert.Util.List.
+Require Import PlutusCert.PlutusIR.Semantics.Static.Theorems.Weakening.
+
+Require Import PlutusCert.PlutusIR.Semantics.TypeSafety.SubstitutionPreservesTyping.SubstituteTCA.
+
+Require Import Lia.
+
+Open Scope string_scope.
+
+(** * Norm: Normalization of STLC *)
+
+(* Hint Constructors multi : core. *)
+
+Declare Custom Entry stlc.
+
+Notation "<{ e }>" := e (e custom stlc at level 99).
+Notation "( x )" := x (in custom stlc, x at level 99).
+Notation "x" := x (in custom stlc at level 0, x constr at level 0).
+Notation "S -> T" := (Kind_Arrow S T) (in custom stlc at level 50, right associativity).
+Notation "x y" := (Ty_App x y) (in custom stlc at level 1, left associativity).
+Notation "\ x : k , y" :=
+  (Ty_Lam x k y) (in custom stlc at level 90, x at level 99,
+                     k custom stlc at level 99,
+                     y custom stlc at level 99,
+                     left associativity).
+Coercion Ty_Var : tyname >-> ty.
+
+Notation "{ x }" := (Ty_Var x) (in custom stlc at level 1, x constr).
+
+Notation "'*'" := Kind_Base (in custom stlc at level 0).
+
+(* ----------------------------------------------------------------- *)
+(* *** Substitution *)
+
+Reserved Notation "'[' x ':=' s ']' t" (in custom stlc at level 20, x constr).
+
+
+Notation "'[' x ':=' s ']' t" := (substituteTCA x s t) (in custom stlc).
+(* ----------------------------------------------------------------- *)
+(** *** Reduction *)
+
+Inductive value : ty -> Prop :=
+  | v_abs : forall x K2 ty1,
+      value <{\x:K2, ty1}>
+  | v_var : forall x,
+      value (Ty_Var x). (* TODO, notation for tyvars?*)
+
+Hint Constructors value : core.
+
+Reserved Notation "ty '-->' ty'" (at level 40).
+
+Inductive step : ty -> ty -> Prop :=
+  | ST_AppAbs : forall x K2 ty1 v2,
+         value v2 ->
+         <{(\x:K2, ty1) v2}> --> <{ [x:=v2]ty1 }>
+  | ST_App1 : forall ty1 ty1' ty2,
+         ty1 --> ty1' ->
+         <{ty1 ty2}> --> <{ty1' ty2}>
+  | ST_App2 : forall v1 ty2 ty2',
+         value v1 ->
+         ty2 --> ty2' ->
+         <{v1 ty2}> --> <{v1  ty2'}>
+
+where "ty '-->' ty'" := (step ty ty').
+
+Hint Constructors step : core.
+
+
+(* ---------------------------------------------------------------------
+Small step*)
+Definition relation (X : Type) := X -> X -> Prop.
+Inductive multi {X : Type} (R : relation X) : relation X :=
+  | multi_refl : forall (x : X), multi R x x
+  | multi_step : forall (x y z : X),
+                    R x y ->
+                    multi R y z ->
+                    multi R x z.
+
+Notation multistep := (multi step).
+Notation "ty1 '-->*' ty2" := (multistep ty1 ty2) (at level 40).
+
+Definition normal_form {X : Type}
+              (R : relation X) (t : X) : Prop :=
+   not (exists t', R t t').
+
+Notation step_normal_form := (normal_form step).
+
+Lemma value__normal : forall t, value t -> step_normal_form t.
+Proof with eauto.
+  intros t H.
+  induction H; intros [t' Hstep]; inversion Hstep.
+Qed.
+
+(* ----------------------------------------------------------------- *)
+(** *** Preservation *)
+
+Theorem preservation : forall t t' T,
+   [] |-* t : T  ->
+   t --> t'  ->
+   [] |-* t' : T.
+Proof with eauto.
+intros t t' T HT. generalize dependent t'.
+remember [] as Gamma.
+induction HT;
+  intros t' HE; subst; inversion HE; subst...
+- apply substituteTCA_preserves_kinding with K1...
+  inversion HT1...
+- (* T_App *)
+  inversion HE; subst...
+  + (* ST_AppAbs *)
+    apply substituteTCA_preserves_kinding with K1...
+    inversion HT1...
+  + 
+    specialize IHHT1 with (ty1').
+    specialize (IHHT1 eq_refl).
+    apply IHHT1 in H0.
+    apply K_App with (K1 := K1); assumption.
+  + apply K_App with (K1 := K1); assumption. 
+- apply K_App with (K1 := K1); [assumption|].
+  apply IHHT2 in H3; [assumption|reflexivity].    
+Qed.
+
+(* ----------------------------------------------------------------- *)
+(** *** Context Invariance *)
+
+(* TODO: This is kind of already defined in Analysis.FreeVars*)
+
+Inductive appears_free_in : string -> ty -> Prop :=
+  | afi_var : forall (x : string),
+      appears_free_in x (Ty_Var x)
+  | afi_app1 : forall x t1 t2,
+      appears_free_in x t1 -> appears_free_in x <{ t1 t2 }>
+  | afi_app2 : forall x t1 t2,
+      appears_free_in x t2 -> appears_free_in x <{ t1 t2 }>
+  | afi_abs : forall x y T11 t12,
+        y <> x  ->
+        appears_free_in x t12 ->
+        appears_free_in x <{ \y : T11, t12 }>
+.
+
+Hint Constructors appears_free_in : core.
+
+Definition closed (t:ty) :=
+  forall x, ~ appears_free_in x t.
+
+Lemma context_invariance : forall Gamma Gamma' t K,
+     Gamma |-* t : K  ->
+     (forall x, appears_free_in x t -> List.lookup x Gamma = List.lookup x Gamma')  ->
+     Gamma' |-* t : K.
+Proof.
+  intros.
+  generalize dependent Gamma'.
+  induction H; intros; eauto 12.
+  - (* T_Var *)
+    apply K_Var. rewrite <- H0; auto.
+  - (* Ty_Fun *)
+    admit.
+  - admit.
+  - admit.
+  - admit.
+  - (* T_Abs *)
+    apply K_Lam.
+    apply IHhas_kind. intros x1 Hafi.
+    
+    (* the only tricky step... *)
+    destruct (eqb_spec X x1); subst.
+    + rewrite lookup_eq.
+      rewrite lookup_eq.
+      reflexivity.
+    + rewrite lookup_neq; [| symmetry; assumption].
+      rewrite lookup_neq; [| symmetry; assumption].
+      auto.
+  - (* Ty_App *)
+    apply K_App with (K1 := K1).
+    + apply IHhas_kind1. intros x1 Hafi.
+      auto.
+    + apply IHhas_kind2. intros x1 Hafi.
+      auto. 
+Admitted.
+
+(* A handy consequence of [eqb_neq]. *)
+Theorem false_eqb_string : forall x y : string,
+   x <> y -> String.eqb x y = false.
+Proof.
+  intros x y. rewrite String.eqb_neq.
+  intros H. apply H. Qed.
+
+Lemma free_in_context : forall x t T Gamma,
+   appears_free_in x t ->
+   Gamma |-* t : T ->
+   exists T', List.lookup x Gamma = Some T'.
+Proof with eauto.
+  intros x t T Gamma Hafi Htyp.
+  induction Htyp; inversion Hafi; subst...
+  - (* T_Abs *)
+    destruct IHHtyp as [T' Hctx]... exists T'.
+    unfold lookup in Hctx.
+    rewrite false_eqb_string in Hctx...
+Qed.
+
+Corollary typable_empty__closed : forall t T,
+    [] |-* t : T  ->
+    closed t.
+Proof.
+  intros. unfold closed. intros x H1.
+  destruct (free_in_context _ _ _ _ H1 H) as [T' C].
+  discriminate C.  
+Qed.
+
+(* ----------------------------------------------------------------- *)
+(** *** Determinism *)
+
+(** To prove determinsm, we introduce a helpful tactic.  It identifies
+    cases in which a value takes a step and solves them by using
+    value__normal.  *)
+
+Ltac solve_by_inverts n :=
+  match goal with | H : ?T |- _ =>
+  match type of T with Prop =>
+    solve [
+      inversion H;
+      match n with S (S (?n')) => subst; solve_by_inverts (S n') end ]
+  end end.
+
+Ltac solve_by_invert :=
+  solve_by_inverts 1.
+
+Ltac solve_by_value_nf :=
+  match goal with | H : value ?v, H' : ?v --> ?v' |- _ =>
+  exfalso; apply value__normal in H; eauto
+  end.
+
+Definition deterministic {X : Type} (R : relation X) :=
+  forall x y1 y2 : X, R x y1 -> R x y2 -> y1 = y2.
+
+Lemma step_deterministic :
+   deterministic step.
+Proof with eauto.
+   unfold deterministic.
+   intros t t' t'' E1 E2.
+   generalize dependent t''.
+   induction E1; intros t'' E2; inversion E2; subst; clear E2;
+   try solve_by_invert; try f_equal; try solve_by_value_nf; eauto.
+Qed.
+
+(* ################################################################# *)
+(** * Normalization *)
+
+(** Now for the actual normalization proof.
+
+    Our goal is to prove that every well-typed term reduces to a
+    normal form.  In fact, it turns out to be convenient to prove
+    something slightly stronger, namely that every well-typed term
+    reduces to a _value_.  This follows from the weaker property
+    anyway via Progress (why?) but otherwise we don't need Progress,
+    and we didn't bother re-proving it above.
+
+    Here's the key definition: *)
+
+Definition halts  (t:ty) : Prop :=  exists t', t -->* t' /\  value t'.
+
+(** A trivial fact: *)
+
+Lemma value_halts : forall v, value v -> halts v.
+Proof.
+  intros v H. unfold halts.
+  exists v. split.
+  - apply multi_refl.
+  - assumption.
+Qed.
+
+(** The key issue in the normalization proof (as in many proofs by
+    induction) is finding a strong enough induction hypothesis.  To
+    this end, we begin by defining, for each type [T], a set [R_T] of
+    closed terms of type [T].  We will specify these sets using a
+    relation [R] and write [R T t] when [t] is in [R_T]. (The sets
+    [R_T] are sometimes called _saturated sets_ or _reducibility
+    candidates_.)
+
+    Here is the definition of [R] for the base language:
+
+    - [R bool t] iff [t] is a closed term of type [bool] and [t] halts
+      in a value
+
+    - [R (T1 -> T2) t] iff [t] is a closed term of type [T1 -> T2] and
+      [t] halts in a value _and_ for any term [s] such that [R T1 s],
+      we have [R T2 (t s)]. *)
+
+(** This definition gives us the strengthened induction hypothesis that we
+    need.  Our primary goal is to show that all _programs_ ---i.e., all
+    closed terms of base type---halt.  But closed terms of base type can
+    contain subterms of functional type, so we need to know something
+    about these as well.  Moreover, it is not enough to know that these
+    subterms halt, because the application of a normalized function to a
+    normalized argument involves a substitution, which may enable more
+    reduction steps.  So we need a stronger condition for terms of
+    functional type: not only should they halt themselves, but, when
+    applied to halting arguments, they should yield halting results.
+
+    The form of [R] is characteristic of the _logical relations_ proof
+    technique.  (Since we are just dealing with unary relations here, we
+    could perhaps more properly say _logical properties_.)  If we want to
+    prove some property [P] of all closed terms of type [A], we proceed by
+    proving, by induction on types, that all terms of type [A] _possess_
+    property [P], all terms of type [A->A] _preserve_ property [P], all
+    terms of type [(A->A)->(A->A)] _preserve the property of preserving_
+    property [P], and so on.  We do this by defining a family of
+    properties, indexed by types.  For the base type [A], the property is
+    just [P].  For functional types, it says that the function should map
+    values satisfying the property at the input type to values satisfying
+    the property at the output type.
+
+    When we come to formalize the definition of [R] in Coq, we hit a
+    problem.  The most obvious formulation would be as a parameterized
+    Inductive proposition like this:
+
+      Inductive R : ty -> tm -> Prop :=
+      | R_bool : forall b t, empty |-- t \in Bool ->
+                      halts t ->
+                      R Bool t
+      | R_arrow : forall T1 T2 t, empty |-- t \in (Arrow T1 T2) ->
+                      halts t ->
+                      (forall s, R T1 s -> R T2 (app t s)) ->
+                      R (Arrow T1 T2) t.
+
+    Unfortunately, Coq rejects this definition because it violates the
+    _strict positivity requirement_ for inductive definitions, which says
+    that the type being defined must not occur to the left of an arrow in
+    the type of a constructor argument. Here, it is the third argument to
+    [R_arrow], namely [(forall s, R T1 s -> R TS (app t s))], and
+    specifically the [R T1 s] part, that violates this rule.  (The
+    outermost arrows separating the constructor arguments don't count when
+    applying this rule; otherwise we could never have genuinely inductive
+    properties at all!)  The reason for the rule is that types defined
+    with non-positive recursion can be used to build non-terminating
+    functions, which as we know would be a disaster for Coq's logical
+    soundness. Even though the relation we want in this case might be
+    perfectly innocent, Coq still rejects it because it fails the
+    positivity test.
+
+    Fortunately, it turns out that we _can_ define [R] using a
+    [Fixpoint]: *)
+
+Fixpoint R (T:kind) (t:ty) : Prop :=
+  [] |-* t : T /\ halts t /\
+  (match T with
+   | <{ * }>  => True
+   | <{ K1 -> K2 }> => (forall s, R K1 s -> R K2 <{t s}> )
+   end).
+
+(** As immediate consequences of this definition, we have that every
+    element of every set [R_T] halts in a value and is closed with type
+    [T] :*)
+
+Lemma R_halts : forall {T} {t}, R T t -> halts t.
+Proof.
+  intros.
+  destruct T; unfold R in H; destruct H as [_ [H _]]; assumption.
+Qed.
+
+Lemma R_typable_empty : forall {T} {t}, R T t -> [] |-* t : T.
+Proof.
+  intros.
+  destruct T; unfold R in H; destruct H as [H _]; assumption.
+Qed.
+
+(** Now we proceed to show the main result, which is that every
+    well-typed term of type [T] is an element of [R_T].  Together with
+    [R_halts], that will show that every well-typed term halts in a
+    value.  *)
+
+(* ================================================================= *)
+(** **  Membership in [R_T] Is Invariant Under Reduction *)
+
+(** We start with a preliminary lemma that shows a kind of strong
+    preservation property, namely that membership in [R_T] is _invariant_
+    under reduction. We will need this property in both directions,
+    i.e., both to show that a term in [R_T] stays in [R_T] when it takes a
+    forward step, and to show that any term that ends up in [R_T] after a
+    step must have been in [R_T] to begin with.
+
+    First of all, an easy preliminary lemma. Note that in the forward
+    direction the proof depends on the fact that our language is
+    determinstic. This lemma might still be true for nondeterministic
+    languages, but the proof would be harder! *)
+
+Lemma step_preserves_halting :
+  forall t t', (t --> t') -> (halts t <-> halts t').
+Proof.
+ intros t t' ST.  unfold halts.
+ split.
+ - (* -> *)
+  intros [t'' [STM V]].
+  destruct STM.
+   + exfalso; apply value__normal in V; eauto.
+   + rewrite (step_deterministic _ _ _ ST H). exists z. split; assumption.
+ - (* <- *)
+  intros [t'0 [STM V]].
+  exists t'0. split; eauto.
+  apply multi_step with (y := t'); assumption.
+Qed.
+
+(** Now the main lemma, which comes in two parts, one for each
+    direction.  Each proceeds by induction on the structure of the type
+    [T]. In fact, this is where we make fundamental use of the
+    structure of types.
+
+    One requirement for staying in [R_T] is to stay in type [T]. In the
+    forward direction, we get this from ordinary type Preservation. *)
+
+Lemma step_preserves_R : forall T t t', (t --> t') -> R T t -> R T t'.
+Proof.
+ induction T;  intros t t' E Rt; unfold R; fold R; unfold R in Rt; fold R in Rt;
+               destruct Rt as [typable_empty_t [halts_t RRt]].
+  (* Bool *)
+  split. eapply preservation; eauto.
+  split. apply (step_preserves_halting _ _ E); eauto.
+  auto.
+  (* Arrow *)
+  split. eapply preservation; eauto.
+  split. apply (step_preserves_halting _ _ E); eauto.
+  intros.
+  eapply IHT2.
+  apply  ST_App1. apply E.
+  apply RRt; auto.
+Qed.
+
+(** The generalization to multiple steps is trivial: *)
+
+Lemma multistep_preserves_R : forall T t t',
+  (t -->* t') -> R T t -> R T t'.
+Proof.
+  intros T t t' STM; induction STM; intros.
+  assumption.
+  apply IHSTM. eapply step_preserves_R. apply H. assumption.
+Qed.
+
+(** In the reverse direction, we must add the fact that [t] has type
+   [T] before stepping as an additional hypothesis. *)
+
+Lemma step_preserves_R' : forall K t t',
+  [] |-* t : K -> (t --> t') -> R K t' -> R K t.
+Proof. (* This proof was not in software foundations *)
+  induction K; intros t t' E Rt; unfold R; fold R. split.
+  - assumption.
+  - destruct H as [_ [Hhalts _]].
+    split; [|reflexivity].
+    apply (step_preserves_halting _ _ Rt).
+    assumption.
+  - split; [|split].
+    + destruct H as [H _].
+      assumption.
+    + apply (step_preserves_halting _ _ Rt). 
+      apply H.
+    + assert (forall s, R K1 s -> <{ t s }> --> <{ t' s }> ) by eauto.
+      assert (forall s, R K1 s -> [] |-* <{ t s }> : K2).
+      {
+        intros s HRK1.
+        induction K1; unfold R in HRK1; fold R in HRK1
+        ; destruct HRK1 as [HRK1 _].
+        - apply K_App with (K1 := Kind_Base); assumption.
+        - apply K_App with (K1 := <{ K1_1 -> K1_2}>); assumption.   
+      }
+      assert (forall s, R K1 s -> [] |-* <{ t' s }> : K2).
+      {
+        intros s HRK1.
+        induction K1; unfold R in HRK1; fold R in HRK1
+        ; destruct HRK1 as [HRK1 _]; destruct H as [H _].
+        - apply K_App with (K1 := Kind_Base); assumption.
+        - apply K_App with (K1 := <{ K1_1 -> K1_2}>); assumption.   
+      }
+      assert (forall s, R K1 s -> R K2 <{t' s}> -> R K2 <{t s}>).
+      {
+        intros s RK1s.
+        apply IHK2 with (t := <{ t s }>) (t' := <{ t' s }>).
+        - apply H1.
+          assumption.
+        - apply H0.
+          assumption. 
+      }
+      destruct H as [_ [_ H]].
+      intros s HRK1.
+      apply H3.
+      * assumption.
+      * apply H.
+        assumption.
+Qed. 
+
+
+    
+  
+
+Lemma multistep_preserves_R' : forall T t t',
+  [] |-* t : T -> (t -->* t') -> R T t' -> R T t.
+Proof.
+  intros T t t' HT STM.
+  induction STM; intros.
+    assumption.
+    eapply step_preserves_R'.  assumption. apply H. apply IHSTM.
+    eapply preservation;  eauto. auto.
+Qed.
+
+(* ================================================================= *)
+(** ** Closed Instances of Terms of Type [t] Belong to [R_T] *)
+
+(** Now we proceed to show that every term of type [T] belongs to
+    [R_T].  Here, the induction will be on typing derivations (it would be
+    surprising to see a proof about well-typed terms that did not
+    somewhere involve induction on typing derivations!).  The only
+    technical difficulty here is in dealing with the abstraction case.
+    Since we are arguing by induction, the demonstration that a term
+    [abs x T1 t2] belongs to [R_(T1->T2)] should involve applying the
+    induction hypothesis to show that [t2] belongs to [R_(T2)].  But
+    [R_(T2)] is defined to be a set of _closed_ terms, while [t2] may
+    contain [x] free, so this does not make sense.
+
+    This problem is resolved by using a standard trick to suitably
+    generalize the induction hypothesis: instead of proving a statement
+    involving a closed term, we generalize it to cover all closed
+    _instances_ of an open term [t].  Informally, the statement of the
+    lemma will look like this:
+
+    If [x1:T1,..xn:Tn |-- t : T] and [v1,...,vn] are values such that
+    [R T1 v1], [R T2 v2], ..., [R Tn vn], then
+    [R T ([x1:=v1][x2:=v2]...[xn:=vn]t)].
+
+    The proof will proceed by induction on the typing derivation
+    [x1:T1,..xn:Tn |-- t : T]; the most interesting case will be the one
+    for abstraction. *)
+
+(* ----------------------------------------------------------------- *)
+(** *** Multisubstitutions, Multi-Extensions, and Instantiations *)
+
+(** However, before we can proceed to formalize the statement and
+    proof of the lemma, we'll need to build some (rather tedious)
+    machinery to deal with the fact that we are performing _multiple_
+    substitutions on term [t] and _multiple_ extensions of the typing
+    context.  In particular, we must be precise about the order in which
+    the substitutions occur and how they act on each other.  Often these
+    details are simply elided in informal paper proofs, but of course Coq
+    won't let us do that. Since here we are substituting closed terms, we
+    don't need to worry about how one substitution might affect the term
+    put in place by another.  But we still do need to worry about the
+    _order_ of substitutions, because it is quite possible for the same
+    identifier to appear multiple times among the [x1,...xn] with
+    different associated [vi] and [Ti].
+
+    To make everything precise, we will assume that environments are
+    extended from left to right, and multiple substitutions are performed
+    from right to left.  To see that this is consistent, suppose we have
+    an environment written as [...,y:bool,...,y:nat,...]  and a
+    corresponding term substitution written as [...[y:=(tbool
+    true)]...[y:=(const 3)]...t].  Since environments are extended from
+    left to right, the binding [y:nat] hides the binding [y:bool]; since
+    substitutions are performed right to left, we do the substitution
+    [y:=(const 3)] first, so that the substitution [y:=(tbool true)] has
+    no effect. Substitution thus correctly preserves the type of the term.
+
+    With these points in mind, the following definitions should make sense.
+
+    A _multisubstitution_ is the result of applying a list of
+    substitutions, which we call an _environment_. *)
+
+(** We need similar machinery to talk about repeated extension of a
+    typing context using a list of (identifier, type) pairs, which we
+    call a _type assignment_. *)
+
+Definition env := list (string * ty).
+Definition kass := list (string * kind).
+
+Open Scope list_scope.
+
+
+Definition mupdate (Gamma : kass) (xts : kass) : kass :=
+  xts ++ Gamma.
+
+(** An _instantiation_ combines a type assignment and a value
+    environment with the same domains, where corresponding elements are
+    in R. *)
+
+Inductive instantiation :  kass -> env -> Prop :=
+| V_nil :
+    instantiation nil nil
+| V_cons : forall x T v c e,
+    value v -> R T v ->
+    instantiation c e ->
+    instantiation ((x,T)::c) ((x,v)::e).
+
+(** We now proceed to prove various properties of these definitions. *)
+
+(* ----------------------------------------------------------------- *)
+(** *** More Substitution Facts *)
+
+(** First we need some additional lemmas on (ordinary) substitution. *)
+
+Lemma vacuous_substitution : forall  t x,
+     ~ appears_free_in x t  ->
+     forall t', <{ [x:=t']t }> = t.
+Proof with eauto.
+  (* FILL IN HERE *) Admitted.
+
+Lemma subst_closed: forall t,
+     closed t  ->
+     forall x t', <{ [x:=t']t }> = t.
+Proof.
+  intros. apply vacuous_substitution. apply H.  Qed.
+
+Lemma subst_not_afi : forall t x v,
+    closed v ->  ~ appears_free_in x <{ [x:=v]t }>.
+Proof with eauto.  (* rather slow this way *)
+  unfold closed, not.
+  induction t; intros x v P A; simpl in A.
+    - (* var *)
+     destruct (eqb_spec x t). 
+      + 
+        funelim (substituteTCA x v (Ty_Var x)); try discriminate.
+        inversion H.
+        symmetry in H1.
+        rewrite <- H1 in Heqcall.
+        rewrite eqb_refl in Heqcall.
+        rewrite <- Heqcall in A.
+        apply P in A.
+        assumption.
+      + funelim (substituteTCA x v (Ty_Var t)); try discriminate.
+        inversion H.
+        rewrite <- H1 in n.
+        rewrite <- eqb_neq in n.
+        rewrite n in Heqcall.
+        rewrite <- Heqcall in A.
+        rewrite -> H in A.
+        inversion A.
+        rewrite <- H1 in H3.
+        rewrite <- eqb_eq in H3.
+        rewrite -> H3 in n.
+        discriminate.
+    - admit.
+    - admit.
+    - admit.
+    - admit.
+    - (* lam *)
+     shelve.
+     
+    - (* app *)
+      funelim (substituteTCA x v <{t1 t2}>); try discriminate.
+      rewrite <- Heqcall in A.
+      inversion A.
+      + apply IHt1 with (x := X) (v := U); [apply P | ].
+        inversion H1.
+        subst...
+      + apply IHt2 with (x := X) (v := U); [apply P | ].
+        inversion H1.
+        subst...     
+Admitted.
+
+Lemma duplicate_subst : forall t' x t v,
+  closed v -> <{ [x:=t]([x:=v]t') }> = <{ [x:=v]t' }>.
+Proof.
+  intros. eapply vacuous_substitution. apply subst_not_afi. assumption.
+Qed.
+
+Lemma subst_tyvar_identity : forall x v t,
+  x <> t -> <{[x := v] {t}}> = <{{t}}>.
+Proof.
+  intros x v t Hneq.
+  funelim (substituteTCA x v (Ty_Var t)); try discriminate.
+  inversion H.
+  rewrite <- H1 in Hneq.
+  apply eqb_neq in Hneq.
+  rewrite Hneq in Heqcall.
+  rewrite <- Heqcall.
+  rewrite -> H1.
+  reflexivity.
+Qed.
+
+Lemma subst_tyvar_value : forall x v ,
+  <{[x := v] {x}}> = <{v}>.
+Proof.
+  intros x v.
+  funelim (substituteTCA x v (Ty_Var x)); try discriminate.
+  inversion H.
+  rewrite H1 in Heqcall.
+  rewrite eqb_refl in Heqcall.
+  rewrite <- Heqcall.
+  reflexivity.
+Qed.
+
+Lemma swap_subst : forall t x x1 v v1,
+    x <> x1 ->
+    closed v -> closed v1 ->
+    <{ [x1:=v1]([x:=v]t) }> = <{ [x:=v]([x1:=v1]t) }>.
+Proof with eauto.
+ induction t; intros; simpl.
+  - (* var *)
+   destruct (eqb_spec x t); destruct (eqb_spec x1 t).
+   + subst. exfalso...
+   + subst. simpl. rewrite subst_closed.
+    * rewrite -> subst_tyvar_identity with (x := x1). reflexivity. assumption. 
+    * rewrite -> subst_tyvar_value.
+      assumption.  
+   + rewrite -> subst_tyvar_identity with (x := x); [|assumption].
+     subst.
+     rewrite subst_tyvar_value.
+     rewrite subst_closed; [reflexivity | assumption].
+   + rewrite subst_tyvar_identity; [|assumption].
+     rewrite subst_tyvar_identity; [|assumption].
+     rewrite subst_tyvar_identity; [|assumption].
+     reflexivity.
+  - admit.
+  - admit.
+  - admit.
+  - admit.
+  - shelve.
+  - shelve.
+Admitted. 
+
+(* ----------------------------------------------------------------- *)
+(** *** Properties of Multi-Substitutions *)
+
+Lemma msubstTCA_closed: forall t, 
+  closed t -> forall ss, msubstTCA ss t = t.
+Proof.
+  induction ss.
+    reflexivity.
+    destruct a. simpl. rewrite subst_closed; assumption.
+Qed.
+
+(** Closed environments are those that contain only closed terms. *)
+
+Fixpoint closed_env (env:env) :=
+  match env with
+  | nil => True
+  | (x,t)::env' => closed t /\ closed_env env'
+  end.
+
+(** Next come a series of lemmas charcterizing how [msubst] of closed terms
+    distributes over [subst] and over each term form *)
+
+Lemma subst_msubstTCA: forall env x v t, closed v -> closed_env env ->
+    msubstTCA env <{ [x:=v]t }> = substituteTCA x v (msubstTCA (drop x env) t).
+Proof.
+  induction env0; intros; auto.
+  destruct a. simpl.
+  inversion H0.
+  destruct (eqb_spec s x).
+  - subst. rewrite duplicate_subst; auto.
+  - simpl. rewrite swap_subst; eauto.
+Qed.
+
+Lemma msubstTCA_var:  forall ss x, closed_env ss ->
+   msubstTCA ss (Ty_Var x) =
+   match lookup x ss with
+   | Some t => t
+   | None => Ty_Var x
+  end.
+Proof.
+  induction ss; intros; [reflexivity|].
+  destruct a as [ax aty].
+  remember (if x =? ax then aty else Ty_Var x) as t'.
+  simpl.
+  destruct (eqb_spec ax x).
+  - subst... rewrite -> subst_tyvar_value.
+    simpl in H; destruct H as [H _].
+    apply msubstTCA_closed.
+    assumption.
+  - rewrite -> subst_tyvar_identity; [|assumption].
+    simpl in H; destruct H as [_ H].
+    rewrite IHss; [reflexivity|assumption]. 
+Qed.
+
+
+(* This is not true because of renaming, but I think I can still kind of use it*)
+Lemma substTCA_abs: forall X1 K1 X2 K2 T,
+  substituteTCA X1 K1 (Ty_Lam X2 K2 T) =
+    if X1 =? X2 then Ty_Lam X2 K2 T else Ty_Lam X2 K2 (substituteTCA X1 K1 T).
+Proof.
+Admitted.
+
+(* TODO: This is not true because of renaming, but let's just assume that it is lol *)
+Lemma msubstTCA_abs: forall ss x T t,
+  msubstTCA ss <{ \ x : T, t }> = Ty_Lam x T (msubstTCA (drop x ss) t).
+Proof.
+  induction ss; intros.
+    reflexivity.
+    destruct a.
+      simpl. destruct (String.eqb s x); simpl; auto.
+Admitted.
+
+(* (* TODO: I also don't think this one holds. 
+  BUt now I do, because msubstTCA is defined as first 
+  substituting the X for the v *)
+  (* I think it holds by the fact that a lambda, after substitution, is still a lambda, and thus a value*)
+  (* So it might be problematic if we start normalising the bodies? But not really, 
+  because we will assume the bodies ar enormalising? *)
+Lemma msubstTCA_beta: forall ss X K ty v,
+  Ty_App (msubstTCA ss (Ty_Lam X K ty)) v -->* msubstTCA ((X, v)::ss) ty.
+Proof.
+Admitted. *)
+
+
+Lemma msubstTCA_app : forall ss t1 t2,
+    msubstTCA ss <{ t1 t2 }> = Ty_App (msubstTCA ss t1) (msubstTCA ss t2).
+Proof.
+ induction ss; intros.
+   reflexivity.
+   destruct a.
+    simpl. rewrite <- IHss. auto.
+Admitted.
+
+(** You'll need similar functions for the other term constructors. *)
+
+(* FILL IN HERE *)
+
+(* ----------------------------------------------------------------- *)
+(** *** Properties of Multi-Extensions *)
+
+(** We need to connect the behavior of type assignments with that of
+    their corresponding contexts. *)
+
+(* Lemma mupdate_lookup : forall (c : kass) (x:string),
+    lookup x c = lookup x c.
+Proof.
+Admitted. TODO: This lemma is not necessary anymore since we use lists instead of partial maps *)
+
+(* Lemma mupdate_drop : forall (c: kass) Gamma x x',
+      mupdate Gamma (drop x c) x'
+    = if String.eqb x x' then Gamma x' else mupdate Gamma c x'.
+Proof.
+  induction c; intros.
+  - destruct (eqb_spec x x'); auto.
+  - destruct a. simpl.
+    destruct (eqb_spec s x).
+    + subst. rewrite IHc.
+      unfold update, t_update. destruct (eqb_spec x x'); auto.
+    + simpl. unfold update, t_update. destruct (eqb_spec s x'); auto.
+      subst. rewrite false_eqb_string; congruence.
+Qed. *)
+
+(* ----------------------------------------------------------------- *)
+(** *** Properties of Instantiations *)
+
+(** These are strightforward. *)
+
+Lemma instantiation_domains_match: forall {c} {e},
+    instantiation c e ->
+    forall {x} {T},
+      lookup x c = Some T -> exists t, lookup x e = Some t.
+Proof.
+  intros c e V. induction V; intros x0 T0 C.
+    solve_by_invert.
+    simpl in *.
+    destruct (String.eqb x x0); eauto.
+Qed.
+
+Lemma instantiation_env_closed : forall c e,
+  instantiation c e -> closed_env e.
+Proof.
+  intros c e V; induction V; intros.
+    econstructor.
+    unfold closed_env. fold closed_env.
+    split; [|assumption].
+    eapply typable_empty__closed. eapply R_typable_empty. eauto.
+Qed.
+
+Lemma instantiation_R : forall c e,
+    instantiation c e ->
+    forall x t T,
+      lookup x c = Some T ->
+      lookup x e = Some t -> R T t.
+Proof.
+  intros c e V. induction V; intros x' t' T' G E.
+    solve_by_invert.
+    unfold lookup in *.  destruct (String.eqb x x').
+      inversion G; inversion E; subst.  auto.
+      eauto.
+Qed.
+
+Lemma instantiation_drop : forall c env,
+    instantiation c env ->
+    forall x, instantiation (drop x c) (drop x env).
+Proof.
+  intros c e V. induction V.
+    intros.  simpl.  constructor.
+    intros. unfold drop.
+    destruct (String.eqb x x0); auto. constructor; eauto.
+Qed.
+
+(* ----------------------------------------------------------------- *)
+(** *** Congruence Lemmas on Multistep *)
+
+(** We'll need just a few of these; add them as the demand arises. *)
+
+Lemma multistep_App2 : forall v t t',
+  value v -> (t -->* t') -> <{ v t }> -->* <{ v t' }>.
+Proof.
+  intros v t t' V STM. induction STM.
+   apply multi_refl.
+   eapply multi_step.
+     apply ST_App2; eauto.  auto.
+Qed.
+
+(* FILL IN HERE *)
+
+(* ----------------------------------------------------------------- *)
+(** *** The R Lemma *)
+
+(** We can finally put everything together.
+
+    The key lemma about preservation of typing under substitution can
+    be lifted to multi-substitutions: *)
+
+Lemma msubstTCA_preserves_kinding : forall c e,
+     instantiation c e ->
+     forall Delta ty K, (mupdate Delta c) |-* ty : K ->
+     Delta |-* (msubstTCA e ty) : K.
+Proof.
+    intros c e H. induction H; intros.
+    simpl in H. simpl. auto.
+    simpl in H2.  simpl.
+    apply IHinstantiation.
+    eapply substituteTCA_preserves_kinding; eauto.
+    assert ([] |-* v : T) by apply (R_typable_empty H0).
+    apply Kinding.weakening_empty.
+    assumption.
+Qed.
+
+Theorem multi_R : forall (X : Type) (R : relation X) (x y : X),
+    R x y -> (multi R) x y.
+Proof.
+Admitted.
+
+Theorem multi_trans :
+  forall (X : Type) (R : relation X) (x y z : X),
+      multi R x y ->
+      multi R y z ->
+      multi R x z.
+Proof.
+Admitted.
+
+(* TODO: Should be true (but is it in small step??? ) *)
+(* We could add hypothesis value v, but I don't know if we need it*)
+(* Lemma step_substitution : forall X s v T,
+  s -->* v -> substituteTCA X s T -->* substituteTCA X v T.
+Proof.
+  intros X s v T hstep.
+  induction T.
+  - funelim (substituteTCA X s (Ty_Var t)); try discriminate.
+    inversion H.
+    destruct (eqb_spec X Y).
+    + rewrite <- Heqcall.
+      subst.
+      rewrite subst_tyvar_value.
+      assumption.
+    + subst.
+      rewrite subst_tyvar_identity; [|assumption].
+      rewrite subst_tyvar_identity; [|assumption].
+      apply multi_refl.
+  - shelve.
+  - shelve.
+  - shelve.
+  - shelve.
+  - rewrite substTCA_abs.
+    rewrite substTCA_abs.
+    destruct (eqb_spec X b).
+    + apply multi_refl.
+    +  
+
+
+Admitted.
+
+Lemma multistep_substitution : forall X s v T env,
+  s -->* v -> msubstTCA ((X, s)::env) T -->* msubstTCA ((X, v)::env) T.
+Proof.
+  intros X s v T env0 Hstep.
+  induction T.
+Admitted. *)
+
+(** And at long last, the main lemma. *)
+
+Lemma msubstTCA_R : forall c env ty K,
+    c |-* ty : K ->
+    instantiation c env ->
+    R K (msubstTCA env ty).
+Proof.
+  intros c env0 ty K HT V.
+  generalize dependent env0.
+  (* We need to generalize the hypothesis a bit before setting up the induction. *)
+  remember c as Delta.
+  generalize dependent c.
+  induction HT; intros.
+
+  - (* T_Var *)
+   destruct (instantiation_domains_match V H) as [t P].
+   eapply instantiation_R; eauto.
+   rewrite msubstTCA_var.  rewrite P. auto. eapply instantiation_env_closed; eauto.
+  - shelve.
+  - shelve.
+  - shelve.
+  - shelve.
+  - (* T_Abs *)
+    unfold R. fold R. split; [|split].
+    + apply msubstTCA_preserves_kinding with (c := Δ ); [assumption|].
+      unfold mupdate. 
+      rewrite app_nil_r.
+      apply K_Lam.
+      assumption.
+    + apply value_halts.
+      rewrite msubstTCA_abs. (* TODO: probably we don't even need something that strong?*)
+      apply v_abs. (* NOTE: this will change when we normalise under the lambda*)
+    + 
+     intros.
+     destruct (R_halts H) as [v [P Q]].
+     pose proof (multistep_preserves_R _ _ _ P H).
+     apply multistep_preserves_R' with (t' := msubstTCA ((X, v)::env0) T).
+     (* * apply multistep_preserves_R' with (t' := msubstTCA ((X, v)::env0) T). *)
+     * 
+       apply K_App with (K1 := K1).
+       -- apply msubstTCA_preserves_kinding with (c := Δ).
+        ++ assumption.
+        ++ unfold mupdate. rewrite app_nil_r.
+           apply K_Lam.
+           assumption.
+       -- induction K1; unfold R in H; destruct H as [H _]; assumption.  
+     * 
+       simpl.
+       rewrite subst_msubstTCA.
+       -- rewrite msubstTCA_abs.
+          apply multi_trans with (y := (Ty_App (Ty_Lam X K1 (msubstTCA (drop X env0) T)) v)).
+          ++ apply multistep_App2; [|assumption].
+             apply v_abs. (* NOTE May get more difficult if lambda is no longer a value*)
+          ++ apply multi_R.
+             apply ST_AppAbs.
+             assumption.
+          
+       -- induction K1; unfold R in H0; destruct H0 as [H0 _];
+          apply typable_empty__closed in H0;
+          assumption.
+       -- apply instantiation_env_closed in V.
+          assumption.
+     * apply multistep_preserves_R' with (t' := msubstTCA ((X, v) :: env0) T).
+       -- apply msubstTCA_preserves_kinding with (c := ((X, K1)::Δ)).
+          ++ apply V_cons; assumption.
+             
+          ++ unfold mupdate. rewrite app_nil_r.
+             assumption.
+       -- apply multi_refl. 
+       -- apply IHHT with (c:= ((X, K1)::Δ)); [reflexivity|].
+          apply V_cons; assumption.
+       
+  - (* T_App *)
+    rewrite msubstTCA_app.
+    destruct (IHHT1 c HeqDelta env0 V) as [_ [_ P1]].
+    pose proof (IHHT2 c HeqDelta env0 V) as P2.
+    fold R in P1. auto.
+Admitted.
+
+(* ----------------------------------------------------------------- *)
+(** *** Normalization Theorem *)
+
+(** And the final theorem: *)
+
+Theorem normalization : forall ty K, [] |-* ty : K -> halts ty.
+Proof.
+  intros.
+  replace ty with (msubstTCA nil ty) by reflexivity.
+  apply (@R_halts K).
+  apply (msubstTCA_R nil); eauto.
+  eapply V_nil.
+Qed.
+
+(* 2024-01-02 21:54 *)
+
+
